WIP

cava/Cava/Semantics/WeakEquivalence.v
@@ -28,6 +28,7 @@ Require Import Cava.Util.List.
 Require Import Cava.Util.Tactics.
 Import Circuit.Notations.
 
+(*
 (* Circuit equivalence relation that stipulates an equal output after n timesteps *)
 Definition cequivn {i o} (n : nat) (c1 c2 : Circuit i o) : Prop :=
   (* there exists some relation between the circuit states and a counter... *)
@@ -50,49 +51,120 @@ Definition cequivn {i o} (n : nat) (c1 c2 : Circuit i o) : Prop :=
 
 Lemma cequivn_compose {i t o} n m (a b : Circuit i t) (c d : Circuit t o) :
   cequivn n a b -> cequivn m c d -> cequivn (n + m) (a >==> c) (b >==> d).
-Admitted.
-
-(* count the number of delays on the critical path of a circuit *)
-Fixpoint cpath {i o} (c : Circuit i o) : nat :=
-  match c with
-  | Comb _ => 0
-  | First f => cpath f
-  | Second f => cpath f
-  | Compose f g => cpath f + cpath g
-  | DelayInit _=> 1
-  | LoopInitCE _ body => cpath body
-  end.
-
-Definition cequivn_reflexive {i o} (c : Circuit i o) :
-  is_loop_free c = true -> cequivn (cpath c) c c.
 Proof.
-  induction c; cbn [cpath is_loop_free].
-  { exists (fun i s1 s2 => i = 0 /\ s1 = s2).
-    ssplit; cbn [value step circuit_state]; intros; subst.
-    all:logical_simplify.
-    all:ssplit; try reflexivity.
-    all:discriminate. }
-  { rewrite Bool.andb_true_iff; intros; logical_simplify.
-    apply cequivn_compose; auto. }
-  { admit. (* applies across First *) }
-  { admit. (* applies across Second *) }
-  { discriminate. }
-  { intros. exists (fun i s1 s2 => i <= 1 /\ s1 = s2).
-    cbn [value step circuit_state].
-    ssplit; intros; logical_simplify; subst; ssplit;
-      try reflexivity; try lia. }
+  intros [Rab [Hab1 [Hab2 [Hab3 Hab4]]]].
+  intros [Rcd [Hcd1 [Hcd2 [Hcd3 Hcd4]]]].
+  exists (fun i s1 s2 =>
+       (m < i -> Rab (i - m) (fst s1) (fst s2))
+       /\ (i <= m -> Rcd i (snd s1) (snd s2))).
+  cbn [value circuit_state].
+  ssplit; intros; destruct_products; cbn [fst snd step] in *;
+    repeat
+      lazymatch goal with
+      | H : ?x + ?y <= ?y |- _ =>
+        destruct x; [ | lia ]; autorewrite with natsimpl in *
+      | H : ?x < 1 |- _ =>
+        destruct x; [ clear H | lia ]; autorewrite with natsimpl in *
+      | H1 : ?y < ?x -> _, H2 : ?x <= ?y -> _ |- _ =>
+        destr (x <=? y); [ specialize (H2 ltac:(lia)); clear H1
+                         | specialize (H1 ltac:(lia)); clear H2 ]
+      | H : Rab 1 ?s1 ?s2 |- context [step a ?s1] => erewrite Hab3 by eassumption
+      | H1 : ?x <= ?y, H2 : ?y < S ?x |- _ =>
+        assert (x = y) by lia; subst; clear H1
+      | _ => first
+              [ progress (ssplit; intros)
+              | erewrite Hab2 by lia
+              | apply Hcd2; lia
+              | apply Hab4; [ lia | solve [auto] ]
+              | solve [auto]
+              | lia
+              | rewrite Nat.sub_succ_l in * by lia
+              | progress autorewrite with natsimpl in * ]
+      end.
+Qed.
+
+Lemma cequivn_delays {t} (r1 r2 : value t) : cequivn 1 (DelayInit r1) (DelayInit r2).
+Proof.
+  exists (fun i s1 s2 => i <= 1 /\ s1 = s2). cbn [value step circuit_state].
+  ssplit; intros; logical_simplify; subst; ssplit; try reflexivity; lia.
+Qed.
+
+Lemma cequivn_comb {i o} (f g : value i -> cava (value o)) :
+  (forall x, f x = g x) -> cequivn 0 (Comb f) (Comb g).
+Proof.
+  intro Hfg. exists (fun i s1 s2 => i = 0). cbn [value step circuit_state].
+  ssplit; intros; logical_simplify; subst; ssplit;
+    repeat lazymatch goal with x : unit |- _ => destruct x end;
+    rewrite ?Hfg; try reflexivity; lia.
+Qed.
+
+Instance Symmetric_cequivn {i o} n : Symmetric (@cequivn i o n) | 10.
+Proof.
+  intros x y [R ?]. logical_simplify. exists (fun i sx sy => R i sy sx).
+  ssplit; intros; auto; symmetry; auto.
+Qed.
+
+(* Restriction that states a circuit is cequivn-equivalent to itself for some n;
+   that is, the number of delays betweeen the inputs and each of the outputs is
+   the same. This will not include most circuits with loops. *)
+Definition uniformly_timed {i o} n (c : Circuit i o) : Prop := cequivn n c c.
+
+Definition wequiv {i o} (c1 c2 : Circuit i o) : Prop :=
+  (* either both circuits are non-uniformly timed *)
+  ((forall n, ~ uniformly_timed n c1)
+   /\ (forall n, ~ uniformly_timed n c2))
+  (* ...or both are uniformly timed with the same timing, and they are
+     cequivn-equivalent with respect to that timing *)
+  \/ (exists n, uniformly_timed n c1
+          /\ uniformly_timed n c2
+          /\ cequivn n c1 c2).
+
+Instance Reflexive_wequiv {i o} : Reflexive (@wequiv i o) | 10.
+Proof.
+  repeat intro. cbv [wequiv].
+  (* here's where we need to *decide* if c is uniformly timed or not *)
+
+  (* thing that returns value nat i -> value nat o
+     Compose f g := fun is => match time f is with
+                              | Some ns => utime g ns
+
+   *)
+Qed.
+Instance Symmetric_wequiv {i o} : Symmetric (@wequiv i o) | 10.
+Proof.
+  repeat intro. cbv [wequiv] in *. logical_simplify.
+  symmetry; auto.
+Qed.
+Instance Transitive_wequiv {i o} : Transitive (@wequiv i o) | 10.
+Proof.
+  repeat intro. cbv [wequiv] in *. logical_simplify.
+  (* This relation is not transitive; a non-uniform y could make both preconditions vacuous *)
+  symmetry; auto.
+Qed.
+
+Print Circuit.
+
+(* Circuits with uniform timing characteristics; all outputs have the same
+   number of delays between them and the circuit inputs *)
+Inductive UCircuit `{semantics:Cava} : nat -> type -> type -> Type :=
+| Comb : forall {i o : type}, (value i -> cava (value o)) -> UCircuit 0 i o
+| Compose : forall {i t o n m}, UCircuit n i t -> UCircuit m t o -> UCircuit (n + m) i o
+| Par : forall {i1 i2 o1 o2 n}, UCircuit n i1 o1 -> UCircuit n i2 o2 -> UCircuit n (i1 * i2) (o1 * o2)
+| LoopInitCE : forall {i o s n}, @value combType s -> UCircuit n (i * s) (o * s) -> UCircuit 0 (i * Bit) o
+| DelayInitCE
+
+
+
+
+(* Circuit equivalence relation that declares the circuits produce equivalent
+   outputs for equivalent inputs after a certain number of delays *)
+Definition wequiv {i o} (c1 c2 : Circuit i o) : Prop :=
+  exists n, cequivn n c1 c2.
+
+Global Instance Transitive_wequiv {i o : type} : Transitive (@wequiv i o) | 10.
 Admitted.
 
-(* Circuit equivalence relation that declares the circuits have equal critical
-   paths and, if both are loop-free, then they produce equivalent outputs for
-   equivalent inputs (delayed by the critical path number) *)
-Definition wequiv {i o} (c1 c2 : Circuit i o) : Prop :=
-  cpath c1 = cpath c2
-  /\ (is_loop_free c1 = true ->
-     is_loop_free c2 = true ->
-     cequivn (cpath c1) c1 c2).
-
-Global Instance Equivalence_wequiv: forall {i o : type}, Equivalence (@wequiv i o) | 10.
+Global Instance Symmetric_wequiv {i o : type} : Symmetric (@wequiv i o) | 10.
 Admitted.
 
 Global Instance Proper_Second {i o t : type} :
@@ -109,9 +181,9 @@ Admitted.
 
 Lemma wequiv_delays {t} (r1 r2 : value t) : wequiv (DelayInit r1) (DelayInit r2).
 Proof.
-  cbv [wequiv]. cbn [cpath is_loop_free]. ssplit; [ reflexivity | intros ].
-  intros. exists (fun i s1 s2 => i <= 1 /\ s1 = s2).
+  cbv [wequiv]. exists 1. exists (fun i s1 s2 => i <= 1 /\ s1 = s2).
   cbn [value step circuit_state].
   ssplit; intros; logical_simplify; subst; ssplit;
-    try reflexivity; try lia.
+    try reflexivity; lia.
 Qed.
+*)
