cava/Cava/Lib/CircuitTransformsProperties.v
@@ -16,6 +16,7 @@
 
 Require Import Coq.Classes.Morphisms.
 Require Import coqutil.Tactics.Tactics.
+Require Import ExtLib.Structures.Monad.
 Require Import Cava.Core.Core.
 Require Import Cava.Semantics.Combinational.
 Require Import Cava.Semantics.Equivalence.
@@ -26,7 +27,7 @@ Require Import Cava.Semantics.Simulation.
 Require Import Cava.Lib.CircuitTransforms.
 Require Import Cava.Util.List.
 Require Import Cava.Util.Tactics.
-Import Circuit.Notations.
+Import MonadNotation Circuit.Notations.
 
 Local Ltac simplify :=
   cbn [circuit_state step Id value]; intros;
@@ -34,19 +35,19 @@ Local Ltac simplify :=
   repeat (destruct_pair_let; cbn [fst snd]);
   logical_simplify; simpl_ident; subst.
 
-Lemma First_Id t1 t2 : @cequiv (t1 * t2) (t1 * t2) (First Id) Id.
+Lemma First_Id {t1 t2} : @cequiv (t1 * t2) (t1 * t2) (First Id) Id.
 Proof.
   exists eq. ssplit; [ reflexivity | ]. simplify. ssplit; reflexivity.
 Qed.
 Hint Rewrite @First_Id using solve [eauto] : circuitsimpl.
 
-Lemma Second_Id t1 t2 : @cequiv (t1 * t2) (t1 * t2) (Second Id) Id.
+Lemma Second_Id {t1 t2} : @cequiv (t1 * t2) (t1 * t2) (Second Id) Id.
 Proof.
   exists eq. ssplit; [ reflexivity | ]. simplify. ssplit; reflexivity.
 Qed.
 Hint Rewrite @Second_Id using solve [eauto] : circuitsimpl.
 
-Lemma Compose_Id_l i o c : @cequiv i o (Id >==> c) c.
+Lemma Compose_Id_l {i o} c : @cequiv i o (Id >==> c) c.
 Proof.
   exists (fun (st1 : unit * value (circuit_state c))
        (st2 : value (circuit_state c)) => st1 = (tt, st2)).
@@ -54,7 +55,7 @@ Proof.
 Qed.
 Hint Rewrite @Compose_Id_l using solve [eauto] : circuitsimpl.
 
-Lemma Compose_Id_r i o c : @cequiv i o (c >==> Id) c.
+Lemma Compose_Id_r {i o} c : @cequiv i o (c >==> Id) c.
 Proof.
   exists (fun (st1 : value (circuit_state c) * unit)
        (st2 : value (circuit_state c)) => st1 = (st2, tt)).
@@ -62,7 +63,7 @@ Proof.
 Qed.
 Hint Rewrite @Compose_Id_r using solve [eauto] : circuitsimpl.
 
-Lemma Compose_assoc A B C D
+Lemma Compose_assoc {A B C D}
       (f : Circuit A B) (g : Circuit B C) (h : Circuit C D) :
   cequiv (f >==> (g >==> h)) (f >==> g >==> h).
 Proof.
@@ -71,22 +72,23 @@ Proof.
        st1 = (fst (fst st2), (snd (fst st2), snd st2))).
   ssplit; [ reflexivity | ]. simplify. ssplit; reflexivity.
 Qed.
+Hint Rewrite @Compose_assoc : circuitsimpl.
 
-Lemma First_Compose A B C D (f : Circuit A B) (g : Circuit B C) :
+Lemma First_Compose {A B C D} (f : Circuit A B) (g : Circuit B C) :
   @cequiv (A * D) (C * D) (First (f >==> g)) (First f >==> First g).
 Proof.
   exists eq. ssplit; [ reflexivity | ]. simplify. ssplit; reflexivity.
 Qed.
 Hint Rewrite @First_Compose using solve [eauto] : circuitsimpl.
 
-Lemma Second_Compose A B C D (f : Circuit A B) (g : Circuit B C) :
+Lemma Second_Compose {A B C D} (f : Circuit A B) (g : Circuit B C) :
   @cequiv (D * A) (D * C) (Second (f >==> g)) (Second f >==> Second g).
 Proof.
   exists eq. ssplit; [ reflexivity | ]. simplify. ssplit; reflexivity.
 Qed.
 Hint Rewrite @Second_Compose using solve [eauto] : circuitsimpl.
 
-Lemma LoopInitCE_First_r A B C (s : SignalType) reset
+Lemma LoopInitCE_First_r {A B C} (s : SignalType) reset
       (body : Circuit (A * s) (B * s)) (f : Circuit B C) :
   cequiv (LoopInitCE reset (body >==> First f)) (LoopInitCE reset body >==> f).
 Proof.
@@ -97,7 +99,7 @@ Proof.
 Qed.
 Hint Rewrite @LoopInitCE_First_r using solve [eauto] : push_loop.
 
-Lemma LoopInit_First_r A B C (s : SignalType) reset
+Lemma LoopInit_First_r {A B C} (s : SignalType) reset
       (body : Circuit (A * s) (B * s)) (f : Circuit B C) :
   cequiv (LoopInit reset (body >==> First f)) (LoopInit reset body >==> f).
 Proof.
@@ -105,19 +107,19 @@ Proof.
 Qed.
 Hint Rewrite @LoopInit_First_r using solve [eauto] : push_loop.
 
-Lemma LoopCE_First_r A B C (s : SignalType)
+Lemma LoopCE_First_r {A B C} (s : SignalType)
       (body : Circuit (A * s) (B * s)) (f : Circuit B C) :
   cequiv (LoopCE (body >==> First f)) (LoopCE body >==> f).
 Proof. apply LoopInitCE_First_r. Qed.
 Hint Rewrite @LoopCE_First_r using solve [eauto] : push_loop.
 
-Lemma Loop_First_r A B C (s : SignalType)
+Lemma Loop_First_r {A B C} (s : SignalType)
       (body : Circuit (A * s) (B * s)) (f : Circuit B C) :
   cequiv (Loop (body >==> First f)) (Loop body >==> f).
 Proof. apply LoopInit_First_r. Qed.
 Hint Rewrite @Loop_First_r using solve [eauto] : push_loop.
 
-Lemma simulate_Id t input : simulate (i:=t) Id input = input.
+Lemma simulate_Id {t} input : simulate (i:=t) Id input = input.
 Proof.
   cbv [Id]; autorewrite with push_simulate.
   apply List.map_id_ext; intros.
@@ -125,7 +127,7 @@ Proof.
 Qed.
 Hint Rewrite @simulate_Id using solve [eauto] : push_simulate.
 
-Lemma simulate_Par A B C D c1 c2 input :
+Lemma simulate_Par {A B C D} c1 c2 input :
   simulate (@Par _ _ A B C D c1 c2) input
   = combine (simulate c1 (map fst input))
             (simulate c2 (map snd input)).
@@ -144,60 +146,68 @@ Proof.
   reflexivity.
 Qed.
 
-Lemma First_Id_w t1 t2 : @wequiv (t1 * t2) (t1 * t2) (First Id) Id.
+Lemma Par_Id_l {i o t} (f : Circuit i o) : cequiv (Par f (Id (t:=t))) (First f).
+Proof. cbv [Par]. autorewrite with circuitsimpl. reflexivity. Qed.
+Hint Rewrite @Par_Id_l using solve [eauto] : circuitsimpl.
+
+Lemma Par_Id_r {i o t} (f : Circuit i o) : cequiv (Par (Id (t:=t)) f) (Second f).
+Proof. cbv [Par]. autorewrite with circuitsimpl. reflexivity. Qed.
+Hint Rewrite @Par_Id_r using solve [eauto] : circuitsimpl.
+
+Lemma Second_Comb {i o t} f :
+  cequiv (Second (Comb f)) (Comb (i:=t*i) (o:=t*o) (fun x => (fst x, f (snd x)))).
 Proof.
-  split; [ reflexivity | ]; intros.
-  cbn [cpath Id].
-  exists (fun i s1 s2 => i = 0 /\ s1 = s2); cbn [step circuit_state value Id fst snd].
-  simpl_ident. ssplit; intros; destruct_products;
-                 subst; ssplit; try reflexivity; discriminate.
+  exists (fun _ _ => True). ssplit; [ tauto | ].
+  cbn [value circuit_state]; intros. destruct_products.
+  repeat lazymatch goal with x : unit |- _ => destruct x end.
+  ssplit; reflexivity.
 Qed.
-Hint Rewrite @First_Id_w using solve [eauto] : circuitsimplw.
+Hint Rewrite @Second_Comb using solve [eauto] : pull_comb.
 
-Lemma Second_Id_w t1 t2 : @wequiv (t1 * t2) (t1 * t2) (Second Id) Id.
+Lemma First_Comb {i o t} f :
+  cequiv (First (Comb f)) (Comb (i:=i*t) (o:=o*t) (fun x => (f (fst x), snd x))).
 Proof.
-  split; [ reflexivity | ]; intros.
-  cbn [cpath Id].
-  exists (fun i s1 s2 => i = 0 /\ s1 = s2); cbn [step circuit_state value Id fst snd].
-  simpl_ident. ssplit; intros; destruct_products;
-                 subst; ssplit; try reflexivity; discriminate.
+  exists (fun _ _ => True). ssplit; [ tauto | ].
+  cbn [value circuit_state]; intros. destruct_products.
+  repeat lazymatch goal with x : unit |- _ => destruct x end.
+  ssplit; reflexivity.
 Qed.
-Hint Rewrite @Second_Id_w using solve [eauto] : circuitsimplw.
+Hint Rewrite @First_Comb using solve [eauto] : pull_comb.
 
-Lemma Compose_Id_l_w i o c : @wequiv i o (Id >==> c) c.
-Admitted.
-Hint Rewrite @Compose_Id_l_w using solve [eauto] : circuitsimplw.
-
-Lemma Compose_Id_r_w i o c : @wequiv i o (c >==> Id) c.
-Admitted.
-Hint Rewrite @Compose_Id_r_w using solve [eauto] : circuitsimplw.
-
-Lemma Par_Id_w t1 t2 : @wequiv (t1 * t2) (t1 * t2) (Par Id Id) Id.
+Lemma Compose_Comb {i t o} f g :
+  cequiv (@Compose _ _ i t o (Comb f) (Comb g)) (Comb (f >=> g)).
 Proof.
-  cbv [Par]. autorewrite with circuitsimplw. reflexivity.
+  exists (fun _ _ => True). ssplit; [ tauto | ].
+  cbn [value circuit_state]; intros. destruct_products.
+  repeat lazymatch goal with x : unit |- _ => destruct x end.
+  ssplit; reflexivity.
 Qed.
-Hint Rewrite @Par_Id_w using solve [eauto] : circuitsimplw.
+Hint Rewrite @Compose_Comb using solve [eauto] : pull_comb.
 
-Lemma Compose_assoc_w A B C D
-      (f : Circuit A B) (g : Circuit B C) (h : Circuit C D) :
-  wequiv (f >==> (g >==> h)) (f >==> g >==> h).
-Admitted.
-Hint Rewrite @Compose_assoc_w using solve [eauto] : circuitsimplw.
-
-Lemma First_Compose_w A B C D (f : Circuit A B) (g : Circuit B C) :
-  @wequiv (A * D) (C * D) (First (f >==> g)) (First f >==> First g).
-Admitted.
-Hint Rewrite @First_Compose_w using solve [eauto] : circuitsimplw.
-
-Lemma Second_Compose_w A B C D (f : Circuit A B) (g : Circuit B C) :
-  @wequiv (D * A) (D * C) (Second (f >==> g)) (Second f >==> Second g).
-Admitted.
-Hint Rewrite @Second_Compose_w using solve [eauto] : circuitsimplw.
-
-Global Instance Proper_Par_w {A B C D} :
-  Proper (wequiv ==> wequiv ==> wequiv) (@Par _ _ A B C D).
+Lemma Compose_Comb_r {i t1 t2 o} c f g :
+  cequiv (@Compose _ _ i t2 o (@Compose _ _ i t1 t2 c (Comb f)) (Comb g))
+         (c >==> Comb (f >=> g)).
 Proof.
-  cbv [Par]. repeat intro.
-  repeat match goal with H : wequiv _ _ |- _ => rewrite H end.
-  reflexivity.
+  rewrite <-Compose_Comb. autorewrite with circuitsimpl. reflexivity.
+Qed.
+Hint Rewrite @Compose_Comb_r using solve [eauto] : pull_comb.
+
+Lemma First_Second_comm {i1 i2 o1 o2} (c1 : Circuit i1 o1) (c2 : Circuit i2 o2) :
+  cequiv (First c1 >==> Second c2) (Second c2 >==> First c1).
+Proof.
+  exists (fun s1 s2 => s1 = (snd s2, fst s2)).
+  ssplit; [ reflexivity | ]. cbn [value circuit_state].
+  intros; destruct_products. cbn [fst snd] in *.
+  logical_simplify. ssplit; reflexivity.
+Qed.
+Hint Rewrite <- @First_Second_comm using solve [eauto] : circuitsimpl.
+
+Lemma Comb_ext {i o} (f g : value i -> cava (value o)) :
+  (forall x, f x = g x) -> cequiv (Comb f) (Comb g).
+Proof.
+  intro Hfg. exists (fun _ _ => True). ssplit; [ tauto | ].
+  cbn [value circuit_state]; intros. destruct_products.
+  repeat lazymatch goal with x : unit |- _ => destruct x end.
+  cbn [step]. rewrite Hfg.
+  ssplit; [ reflexivity | tauto ].
 Qed.
